Add managed and unmanaged capability tests

extract/Main.hs
@@ -5,16 +5,56 @@ import Test.Hspec
 
 main :: IO ()
 main = hspec $ do
-    describe "Basic tests" $ do
-        it "Unit smoke test" $ do
-            eval (Lit LitUnit)
-              `shouldBe`
-                Right (VUnit, MkLog)
+  describe "Basic tests" $ do
+    it "Unit smoke test" $ do
+      eval (Lit LitUnit)
+        `shouldBe`
+          Right (VUnit, MkLog)
 
-        it "Lambda AddInt smoke test" $ do
-            eval
-              (APP (APP (Bltn AddInt)
-                        (Lit (LitInteger 123)))
-                   (Lit (LitInteger 456)))
-              `shouldBe`
-                Right (VInteger 579,MkLog)
+    it "AddInt smoke test" $ do
+      eval (APP (APP (Bltn AddInt)
+                     (Lit (LitInteger 123)))
+                (Lit (LitInteger 456)))
+        `shouldBe`
+          Right (VInteger 579, MkLog)
+
+    it "SubInt smoke test" $ do
+      eval (APP (APP (Bltn SubInt)
+                     (Lit (LitInteger 456)))
+                (Lit (LitInteger 123)))
+        `shouldBe`
+          Right (VInteger 333, MkLog)
+
+    it "Unmanaged capability smoke test" $ do
+      let cap = Capability (Symbol "ALLOW_USER")
+                           (Lit (LitString "john"))
+                           (Lit LitUnit)
+      evalInModule "module"
+        (WithCapability
+          (Symbol "module")
+          (LAM (Lit LitUnit))
+          (LAM (Lit LitUnit))
+          cap
+          (RequireCapability cap))
+        `shouldBe`
+          Right (VUnit, MkLog)
+
+    it "Managed capability smoke test" $ do
+      let cap n =
+            Capability (Symbol "TRANSFER")
+                       (Pair (Lit (LitString "john"))
+                             (Lit (LitString "jose")))
+                       (Lit (LitInteger n))
+      evalInModule "module"
+        (Seq
+          (InstallCapability (cap 100))
+          (WithCapability
+            (Symbol "module")
+            (LAM (Lit LitUnit))
+            (LAM (APP (APP (Bltn SubInt)
+                           (Fst (VAR ZV)))
+                      (Snd (VAR ZV))))
+            (cap 50)
+            (RequireCapability (cap 50))))
+        `shouldBe`
+          Right (VUnit, MkLog)
