extract/src/Pact.hs
@@ -12,7 +12,9 @@ module Pact (
   module Lang,
   module Types,
   evalExp,
-  eval
+  evalInModuleExp,
+  eval,
+  evalInModule
 
 ) where
 
@@ -25,15 +27,15 @@ import Value hiding (Any, __, reifyTy)
 import Ty hiding (__)
 import qualified CapabilityType
 
-deriving instance Show Ty.PrimType
-deriving instance Show Ty.Ty
-deriving instance Show Value.ValueTy
-deriving instance Show Value.Value
-deriving instance Show Exp.Err
-deriving instance Show CapabilityType.CapSig
-deriving instance Show CapabilityType.CapError
-deriving instance Show Lang.Err
-deriving instance Show Lang.PactLog
+-- deriving instance Show Ty.PrimType
+-- deriving instance Show Ty.Ty
+-- deriving instance Show Value.ValueTy
+-- deriving instance Show Value.Value
+-- deriving instance Show Exp.Err
+-- deriving instance Show CapabilityType.CapSig
+-- deriving instance Show CapabilityType.CapError
+-- deriving instance Show Lang.Err
+-- deriving instance Show Lang.PactLog
 
 deriving instance Eq Ty.PrimType
 deriving instance Eq Ty.Ty
@@ -45,8 +47,9 @@ deriving instance Eq CapabilityType.CapError
 deriving instance Eq Lang.Err
 deriving instance Eq Lang.PactLog
 
-instance Show CapabilityType.Cap where
-  show (CapabilityType.Token name _ _) = "Cap " ++ name
+-- instance Show CapabilityType.Cap where
+--   show (CapabilityType.Token name _x _y) =
+--     "(Cap " ++ name ++ " " ++ "_" ++ " " ++ "_" ++ ")"
 
 instance Eq CapabilityType.Cap where
   CapabilityType.Token name1 _ _ == CapabilityType.Token name2 _ _ =
@@ -58,8 +61,22 @@ evalExp
   -> Either Lang.Err (Value.Value, Lang.PactLog)
 evalExp = Eval.eval
 
+evalInModuleExp
+  :: String
+  -> Ty.Ty
+  -> Exp.Exp
+  -> Either Lang.Err (Value.Value, Lang.PactLog)
+evalInModuleExp = Eval.evalInModule
+
 eval
   :: forall t. ReifyTy t
   => Types.Exp '[] t
   -> Either Lang.Err (Value.Value, Lang.PactLog)
 eval e = evalExp (reifyTy @t) (forgetExp e)
+
+evalInModule
+  :: forall t. ReifyTy t
+  => String
+  -> Types.Exp '[] t
+  -> Either Lang.Err (Value.Value, Lang.PactLog)
+evalInModule name e = evalInModuleExp name (reifyTy @t) (forgetExp e)
