src/Eval.v
@@ -1,5 +1,6 @@
 Require Import
   Coq.ZArith.ZArith
+  Hask.Control.Lens
   Hask.Control.Monad
   Hask.Data.Either
   Pact.ilist
@@ -19,6 +20,18 @@ Import ListNotations.
 
 Definition eval `(e : Exp [] τ) : Err + (Value τ * PactLog) :=
   match SemExp e tt newPactEnv newPactState newPactLog with
+  | inl err => inl err
+  | inr (result, (_finalState, log)) =>
+      match Reifiable τ with
+      | None   => inl (Err_CannotReify τ)
+      | Some H => inr (reify result H, log)
+      end
+  end.
+
+Definition evalInModule (modname : string) `(e : Exp [] τ) :
+  Err + (Value τ * PactLog) :=
+  match SemExp e tt (newPactEnv &+ context %~ cons (InModule modname))
+               newPactState newPactLog with
   | inl err => inl err
   | inr (result, (_finalState, log)) =>
       match Reifiable τ with
